\section*{Logarithm Identity Practice}
Basic logarithm properties:

Power
$$\log a^b= b\log a$$
Product
$$\log ab = \log a + \log b$$
Quotient
$$\log \frac{a}{b} = \log (ab^-1) = \log a + \log b^{-1} = \log a - \log b$$

Change of Base

$$\log_b a = \frac{\log_d a}{\log_d b}$$

$$\log_b a = \frac{1}{\log_a b}$$

\begin{questions}

\question

Suppose $\log a=5$, $\log b=\frac{3}{2}$ and $\log c=\frac{3}{4}$. 

\textbf{Example:} $\log bc = \log b + \log c = \frac{3}{2} + \frac{3}{4}= \frac{9}{4}$

Use log identities to calculate:

\begin{parts}

\part $\log(ab)$
\begin{solution}[.75in]
  $\log (ab) = \log a + \log b = 5 + \frac{3}{2} = \frac{13}{2}$
\end{solution}
\part $\displaystyle{\log\left(\frac{b}{c}\right)}$
\begin{solution}[.75in]
  $$\log\left(\frac{b}{c}\right) = \log b - \log c = \frac{3}{2} - \frac{3}{4} = \frac{3}{4}$$
\end{solution}
\part $\log(c^4)$
\begin{solution}[.75in]
  $\log(c^4) = 4 \log(c) = 4\cdot \frac{3}{4} = 3$
\end{solution}
\part $\log\sqrt{b}$
\vspace{.3in}
\begin{solution}[.75in]
  $$\log(\sqrt{b} = \log(b^\frac{1}{2}) = \frac{1}{2} \cdot \frac{3}{2} = \frac{3}{4}$$
\end{solution}
\part $\displaystyle{\log\left(\frac{a}{c}\right)^6}$
\vspace{.3in}
\begin{solution}[.75in]
  $$\log\left(\frac{a}{c}\right)^6 = 6\log(\left(\frac{a}{c}\right) = 6 (\log a - \log c) = 6 \left(5 - \frac{3}{4}\right) = 6\frac{23}{4} = \frac{69}{2}$$
\end{solution}

\end{parts}
\end{questions}
