\section*{Derivative Review. Products}
Basic Formulas
\begin{equation}
  \begin{aligned}
    \frac{d}{dx} \left(f(x)g(x)\right) &= g(x)\frac{d}{dx} f(x)+f(x)\frac{d}{dx} g(x) \\
    \noalign{\vspace{1 em}or if}
    h(x) &= f(x)g(x) \\
    \noalign{then}
    h'(x) &= f^\prime(x)g(x)+f(x)g^\prime(x) \\
  \end{aligned}
\end{equation}

\begin{questions}
\question
Calculate the derivative of f(x)=(x+3)(x-2) two ways. Use the product rule and expand the polynomial
\begin{solution}[1.5in]
  Product rule:
  $$f^\prime(x)=1\cdot(x-2)+1\cdot(x+3) = 2x+1$$
  Multiply out the polynomial
  $$f(x)=x^2+x-6$$
  so
  $$f^\prime(x)=2x+1$$
\end{solution}
\question
Calculate the derviative of $x\sin(x)$
\begin{solution}[1.5in]
  $\cos(x)+x\sin(x)$
\end{solution}
\question
(2 points) Given the table

  \begin{tabular}{c|cccccc}
    \hline
    & $f(x)$ & $f^\prime(x)$ & $g(x)$ & $g'(x)$ & $h(x)$ & $h^\prime(x)$ \\
    \hline
    1& 1 & 3 & 9 & 4 & 7 & 17 \\
    \hline
    5 &3 & 6 & 7 & 5 & 4 & 1 \\
    \hline
    -3 &3 & 5 & 4 & 5 & 7& 7  \\
    \hline
  \end{tabular}
  \vspace{1em}
  \begin{parts}
    \part Calculate $k'(1)$ where $k(x) = f(x)g(x)$.
    \begin{solution}[.5in]
      $k'(x)=f'(x)g(x)+f(x)g'(x)$ so $k'(1)= 3\cdot9+1\cdot4=27+4=\fbox{31}$
    \end{solution}
    \part Calculate $k'(5)$ where $k(x) = h(x)f(x)$.
    \begin{solution}[.5in]
      $k'(x)=h'(x)f(x)+h(x)f'(x)$ so $k'(5)= 1\cdot3+4\cdot6=3+24=\fbox{27}$
    \end{solution}
    \part Calculate $k'(-3)$ where $k(x) = f(x)g(x)h(x)$.
    \begin{solution}[.5in]
      Let $\ell(x)=f(x)g(x)$ then $\ell(-3)=3\cdot 4 = 12$ and $\ell'(-3) = 3\cdot 5+5\cdot 4 = 35$
      $k'(x)=h'(x)\ell(x)+h(x)\ell'(x)$ so $k'(-3)= 7\cdot12+7\cdot35=84+245=\fbox{329}$
    \end{solution}
  \end{parts}
\end{questions}
